Addressing change requests from the last meeting

Coq/CSP.v
@@ -7,12 +7,12 @@ Open Scope string_scope.
 
 (** TYPE DEFINITIONS **)
 
-(* TODO Check if it is okay to define the "event" type as a notation instead of an inductive type. *)
-
 Notation event := string.
 
-(* Inductive event : Type :=
-  | Event (name : string). *)
+Inductive event_tau_tick :=
+  | Event (e : event)
+  | Tau
+  | Tick.
 
 Inductive alphabet : Type :=
   | Alphabet (events : set event).
@@ -38,31 +38,28 @@ Inductive proc_def : Type :=
 Inductive specification : Type :=
   | Spec (ch_list : list channel) (proc_list : list proc_def).
 
-Fixpoint proc_eq (P Q : proc_body) : Prop :=
-  match P, Q with
-  | SKIP, SKIP => True
-  | STOP, STOP => True
-  | ProcRef a, ProcRef b => eq a b
-  | ProcPrefix a A, ProcPrefix b B => eq a b /\ proc_eq A B
-  (* | ProcExtChoice A B, ProcExtChoice X Y => proc_eq A B /\ proc_eq X Y
-  | ProcIntChoice A B, ProcIntChoice X Y => proc_eq A B /\ proc_eq X Y
-  | ProcAlphaParallel A B K L, ProcAlphaParallel X Y M N => proc_eq A B /\ proc_eq X Y /\ eq K M /\ eq L N
-  | ProcGenParallel A B K, ProcGenParallel X Y M => proc_eq A B /\ proc_eq X Y /\ eq K M
-  | ProcInterleave A B, ProcInterleave X Y => proc_eq A B /\ proc_eq X Y
-  | ProcSeqComp A B, ProcSeqComp X Y => proc_eq A B /\ proc_eq X Y *)
-  | _, _ => False
-end.
+Fixpoint find_proc_body (proc_list : list proc_def) (proc_name : string) : proc_body :=
+  match proc_list with
+  | [] => STOP
+  | (Proc name body) :: tail => match eqb proc_name name with
+                                | true => body
+                                | false => find_proc_body tail proc_name
+                                end
+  end.
 
-(** NOTATIONS/COERCIONS **)
+Definition get_proc_body (context : specification) (proc_name : string) : proc_body :=
+  match context with
+  | Spec ch_list proc_list => find_proc_body proc_list proc_name
+  end.
 
-Check string_dec.
+(** NOTATIONS/COERCIONS **) 
+
 Definition event_dec := string_dec.
 
-(* Notations for declaring sets of events.
-  TODO Validate the syntax for defining channels and alphabets. *)
-Notation "{ }" := (empty_set event) (format "{ }").
-Notation "{ x }" := (set_add event_dec x (empty_set event)). (* TODO This notation is not working properly. *)
-Notation "{ x , y , .. , z }" := (set_add event_dec x (set_add event_dec y .. (set_add event_dec z (empty_set event)) ..)).
+(* Notations for declaring sets of events. *)
+Notation "{{ }}" := (empty_set event) (format "{{ }}").
+Notation "{{ x }}" := (set_add event_dec x (empty_set event)).
+Notation "{{ x , y , .. , z }}" := (set_add event_dec x (set_add event_dec y .. (set_add event_dec z (empty_set event)) ..)).
 
 (* Process reference (coercion). *)
 Definition str_to_proc_body (s : string) : proc_body := ProcRef s.
@@ -75,14 +72,13 @@ Notation "a --> P" := (ProcPrefix a P) (at level 80, right associativity).
 Notation "P [] Q" := (ProcExtChoice P Q) (at level 90, left associativity).
 (* Internal Choice *)
 Notation "P |~| Q" := (ProcIntChoice P Q) (at level 90, left associativity).
-(* Alphabetised Parallel (TODO This notation is not working properly.) *)
-Notation "P [ A || B ] Q" := (ProcAlphaParallel P Q A B) (at level 90, no associativity).
+(* Alphabetised Parallel (TODO Still not working...) *)
+Notation "P [[ A || B ]] Q" := (ProcAlphaParallel P Q A B) (at level 90, no associativity).
 (* Generalised (or Interface) Parallel *)
 Notation "P [| A |] Q" := (ProcGenParallel P Q A) (at level 90, no associativity).
 (* Interleaving *)
 Notation "P ||| Q" := (ProcInterleave P Q) (at level 90, left associativity).
-(* Sequencial Composition (";" is already defined in list notations)
-  TODO Validate with Gustavo this notation. *)
+(* Sequencial Composition *)
 Notation "P ;; Q" := (ProcSeqComp P Q) (at level 90, left associativity).
 
 (* Example 3.20 (book) using notations. *)
@@ -90,10 +86,10 @@ Definition SPurchase :=
   (
     Spec
     [
-      Channel {"select", "keep", "return"}
-      ; Channel {"cash", "cheque", "card"}
-      ; Channel {"swipe", "sign"}
-      ; Channel {"receipt", "reject"}
+      Channel {{"select", "keep", "return"}}
+      ; Channel {{"cash", "cheque", "card"}}
+      ; Channel {{"swipe", "sign"}}
+      ; Channel {{"receipt", "reject"}}
     ]
 
     [
@@ -107,72 +103,69 @@ Definition SPurchase :=
     ]
   ).
 
-(* TODO: here, "string" is an event in the semantic level, with tick and tau *)
+Compute get_proc_body SPurchase "PURCHASE".
 
-(* TODO: I would prefer proc_body -> event -> proc_body, but this
-         change has an impact in the notation definition before *)
-
-(* TODO Constraint the event sets in the transition rules bellow according to the book.
-  (i.e. whether to include tick and tau events in the alphabet)  *)
+(* TODO Add context (specification) to this type.
+  Revisit the transition rules bellow and check their alphabet. *)
 Reserved Notation "P '//' a '==>' Q" (at level 150, left associativity).
-Inductive sosR : proc_body -> string -> proc_body -> Prop :=
+Inductive sosR : proc_body -> event_tau_tick -> proc_body -> Prop :=
   (* Prefix *)
-  | prefix_rule (P Q : proc_body) (a : string) :
-      (a --> P) // a ==> Q
-  (* Reference. TODO This rule relies on the whether equality of process is decidable (and it should be). *)
-  | reference_rule (P : proc_body) :
-      forall (P' N : proc_body) (a : string), (P // a ==> P') /\ (proc_eq P N) -> N // a ==> P'
+  | prefix_rule (P Q : proc_body) (a : event) :
+      (a --> P) // Event a ==> Q
+  (* Reference *)
+  | reference_rule (P : proc_body) (name : string) :
+      eq P (ProcRef name) -> P // Tau ==> P (*TODO (get_proc_body spec name) *)
   (* External Choice *)
   | ext_choice_left_rule (P Q : proc_body) :
-      forall (P' : proc_body) (a : string), (P // a ==> P') -> (P [] Q // a ==> P')
+      forall (P' : proc_body) (a : event), (P // Event a ==> P') -> (P [] Q // Event a ==> P')
   | ext_choice_right_rule (P Q : proc_body) :
-      forall (P' : proc_body) (a : string), (P // a ==> P') -> (Q [] P // a ==> P')
+      forall (P' : proc_body) (a : event), (P // Event a ==> P') -> (Q [] P // Event a ==> P')
   (* Internal Choice. TODO This definition is not working properly. *)
   | int_choice_left_rule (P Q : proc_body) :
-      forall (tau : string), P |~| Q // tau ==> P
+      forall (tau : string), P |~| Q // Tau ==> P
   | int_choice_right_rule (P Q : proc_body) (tau : string) :
-      forall (tau : string), P |~| Q // tau ==> Q
+      forall (tau : string), P |~| Q // Tau ==> Q
   (* Alphabetised Parallel *)
   | alpha_parall_indep_left_rule (P Q : proc_body) (A B : alphabet) :
-      forall (P' : proc_body) (a : string), (P // a ==> P') -> (ProcAlphaParallel P Q A B) // a ==> (ProcAlphaParallel P' Q A B)
+      forall (P' : proc_body) (a : event), (P // Event a ==> P') -> (ProcAlphaParallel P Q A B) // Event a ==> (ProcAlphaParallel P' Q A B)
   | alpha_parall_indep_right_rule (P Q : proc_body) (A B : alphabet) :
-      forall (P' : proc_body) (a : string), (P // a ==> P') -> (ProcAlphaParallel Q P A B) // a ==> (ProcAlphaParallel Q P' A B)
+      forall (P' : proc_body) (a : event), (P // Event a ==> P') -> (ProcAlphaParallel Q P A B) // Event a ==> (ProcAlphaParallel Q P' A B)
   | alpha_parall_joint_rule (P Q : proc_body) (A B : alphabet) :
-      forall (P' Q' : proc_body) (a : string), (P // a ==> P') -> (Q // a ==> Q') -> (ProcAlphaParallel P Q A B) // a ==> (ProcAlphaParallel P' Q' A B)
+      forall (P' Q' : proc_body) (a : event), (P // Event a ==> P') -> (Q // Event a ==> Q') -> (ProcAlphaParallel P Q A B) // Event a ==> (ProcAlphaParallel P' Q' A B)
   (* Generalised Parallel *)
   | gener_parall_indep_left_rule (P Q : proc_body) (A : alphabet) :
-      forall (P' : proc_body) (a : string), (P // a ==> P') -> P [| A |] Q // a ==> P' [| A |] Q
+      forall (P' : proc_body) (a : event), (P // Event a ==> P') -> P [| A |] Q // Event a ==> P' [| A |] Q
   | gener_parall_indep_right_rule (P Q : proc_body) (A : alphabet) :
-    forall (P' : proc_body) (a : string), (P // a ==> P') -> Q [| A |] P // a ==> Q [| A |] P'
+    forall (P' : proc_body) (a : event), (P // Event a ==> P') -> Q [| A |] P // Event a ==> Q [| A |] P'
   | gener_parall_joint_rule (P Q : proc_body) (A : alphabet) :
-      forall (P' Q' : proc_body) (a : string), (P // a ==> P') -> (Q // a ==> Q') -> P [| A |] Q // a ==> P' [| A |] Q'
+      forall (P' Q' : proc_body) (a : event), (P // Event a ==> P') -> (Q // Event a ==> Q') -> P [| A |] Q // Event a ==> P' [| A |] Q'
   (* Interleave *)
   | interleave_left_rule (P Q : proc_body) :
-      forall (P' : proc_body) (a : string), (P // a ==> P') -> P ||| Q // a ==> P' ||| Q
+      forall (P' : proc_body) (a : event), (P // Event a ==> P') -> P ||| Q // Event a ==> P' ||| Q
   | interleave_right_rule (P Q : proc_body) :
-      forall (P' : proc_body) (a : string), (P // a ==> P') -> Q ||| P // a ==> Q ||| P'
+      forall (P' : proc_body) (a : event), (P // Event a ==> P') -> Q ||| P // Event a ==> Q ||| P'
   | interleave_tick_rule (P Q : proc_body) :
       (* TODO Check if there is indeed a conjuction in this transition rule. *)
-      forall (P' Q' : proc_body) (tick : string), (P // tick ==> P') /\ (Q // tick ==> Q') -> P ||| Q // tick ==> P' ||| Q'
+      forall (P' Q' : proc_body), (P // Tick ==> P') /\ (Q // Tick ==> Q') -> P ||| Q // Tick ==> P' ||| Q'
   (* Sequential Composition *)
   | seq_comp_rule (P Q : proc_body) :
-      forall (P' : proc_body) (a : string), (P // a ==> P') -> P ;; Q // a ==> P' ;; Q
+      forall (P' : proc_body) (a : event), (P // Event a ==> P') -> P ;; Q // Event a ==> P' ;; Q
   | seq_comp_tick_rule (P Q : proc_body) :
-      forall (P' : proc_body) (tick tau : string), (P // tick ==> P') -> P ;; Q // tau ==> Q
+      forall (P' : proc_body), (P // Tick ==> P') -> P ;; Q // Tau ==> Q
   where "P '//' a '==>' Q" := (sosR P a Q).
 
 Reserved Notation "P '///' t '==>' Q" (at level 150, left associativity).
-Inductive sosStarR : proc_body -> list string -> proc_body -> Prop :=
+Inductive sosStarR : proc_body -> list event_tau_tick -> proc_body -> Prop :=
   | sos_empty_rule (P : proc_body) :
       P /// nil ==> P
-  | sos_transitive_rule (P R Q : proc_body) (head : string) (tail : list string) :
+  | sos_transitive_rule (P R Q : proc_body) (head : event_tau_tick) (tail : list event_tau_tick) :
       (P // head ==> R) -> (R /// tail ==> Q) -> (P /// (head :: tail) ==> Q)
   where "P '///' t '==>' Q" := (sosStarR P t Q).
   
-Definition traceBodyR (body : proc_body) (t : list string) :=
+Definition traceBodyR (body : proc_body) (t : list event_tau_tick) :=
   exists (body' : proc_body), body /// t ==> body'.
   
-Definition traceR (P : proc_def) (t : list string) :=
+Definition traceR (P : proc_def) (t : list event_tau_tick) :=
   match P with
   | Proc name body => traceBodyR body t
   end.
@@ -188,7 +181,7 @@ Proof.
   apply sos_empty_rule.
 Qed.
 
-Example PRINTER0_trace1 : traceR PRINTER0 ["accept"].
+Example PRINTER0_trace1 : traceR PRINTER0 [Event "accept"].
 Proof.
   unfold traceR. simpl.
   exists ("print" --> STOP).
@@ -197,7 +190,7 @@ Proof.
   - apply sos_empty_rule.
 Qed.
 
-Example PRINTER0_trace2 : traceR PRINTER0 ["accept" ; "print"].
+Example PRINTER0_trace2 : traceR PRINTER0 [Event "accept" ; Event "print"].
 Proof.
   unfold traceR. simpl.
   exists (STOP).
@@ -219,7 +212,7 @@ Qed.
    - https://coq-club.inria.narkive.com/PQalG3f4/how-to-solve-trivial-evars-automatically-so-that-they-don-t-get-shelved
 *)
 
-Example PRINTER0_trace2' : traceR PRINTER0 ["accept" ; "print"].
+Example PRINTER0_trace2' : traceR PRINTER0 [Event "accept" ; Event "print"].
 Proof.
   unfold traceR. simpl.
   exists (STOP).
@@ -233,7 +226,7 @@ Qed.
 
 Definition CHOOSE := "CHOOSE" ::= "select" --> ("keep" --> SKIP 
                                                 [] "return" --> "CHOOSE").
-Example CHOOSE_trace1 : traceR CHOOSE ["select" ; "keep"].
+Example CHOOSE_trace1 : traceR CHOOSE [Event "select" ; Event "keep"].
 Proof.
   unfold traceR. simpl.
   exists (SKIP).
@@ -245,7 +238,7 @@ Proof.
     * apply sos_empty_rule.
 Qed.
 
-Example CHOOSE_trace2 : traceR CHOOSE ["select" ; "return"].
+Example CHOOSE_trace2 : traceR CHOOSE [Event "select" ; Event "return"].
 Proof.
   unfold traceR. simpl.
   exists ("CHOOSE").
@@ -263,18 +256,17 @@ Definition PETE := "PETE" ::= "lift_piano" --> "PETE"
 Definition DAVE := "DAVE" ::= "lift_piano" --> "DAVE"
                               |~| "lift_table" --> "DAVE".
 
-Definition TEAM := "TEAM" ::= "PETE" [| Alphabet {"lift_piano", "lift_table"} |] "DAVE".
+Definition TEAM := "TEAM" ::= "PETE" [| Alphabet {{"lift_piano", "lift_table"}} |] "DAVE".
 
-Example TEAM_trace1 : traceR TEAM ["lift_piano"].
+(* TODO Revisit once the reference_rule is defined. *)
+Example TEAM_trace1 : traceR TEAM [Event "lift_piano"].
 Proof.
   unfold traceR. simpl.
   exists ("TEAM").
-  apply sos_transitive_rule with (R := "PETE" [| Alphabet {"lift_piano", "lift_table"} |] "DAVE").
-  - apply gener_parall_joint_rule.
-    * apply reference_rule with (P := "lift_piano" --> "PETE" |~| "lift_table" --> "PETE"). split.
-      + Fail eapply int_choice_left_rule. Abort.
+  apply sos_transitive_rule with (R := "PETE" [| Alphabet {{"lift_piano", "lift_table"}} |] "DAVE").
+  - apply gener_parall_joint_rule. Abort.
 
-Example LIGHT_trace1 : traceR ("LIGHT" ::= "on" --> "off" --> "LIGHT") ["on" ; "off" ; "on"].
+Example LIGHT_trace1 : traceR ("LIGHT" ::= "on" --> "off" --> "LIGHT") [Event "on" ; Event "off" ; Event "on"].
 Proof.
   unfold traceR. simpl.
   exists ("off" --> "LIGHT").
@@ -287,7 +279,6 @@ Proof.
       + apply sos_empty_rule.
 Qed.
 
-(* TODO Mention the workaround made here (define proc_body's instead of proc_def's) and why. *)
 Definition PUMP1 := "lift_nozzle_1" --> "READY1".
 Definition READY1 := "replace_nozzle_1" --> "PUMP1"
                       [] "depress_trigger_1" --> "release_trigger_1" --> "READY1".
@@ -296,8 +287,9 @@ Definition READY2 := "replace_nozzle_2" --> "PUMP2"
                       [] "depress_trigger_2" --> "release_trigger_2" --> "READY2".
 Definition FORECOURT := "FORECOURT" ::= PUMP1 ||| PUMP2.
 
-Example FORECOURT_trace1 : traceR FORECOURT ["lift_nozzle_1" ; "depress_trigger_1" ; "lift_nozzle_2" ;
-                                  "depress_trigger_2" ; "release_trigger_2"].
+(* TODO Revisit once the reference_rule is defined. *)
+Example FORECOURT_trace1 : traceR FORECOURT [Event "lift_nozzle_1" ; Event "depress_trigger_1" ; Event "lift_nozzle_2" ;
+                                            Event "depress_trigger_2" ; Event "release_trigger_2"].
 Proof.
   unfold traceR. simpl.
   exists("release_trigger_1" --> READY1 ||| READY2).
